share/everparse/tests/lowparse/LowParseExample9.fst
@@ -3,16 +3,18 @@ module LowParseExample9
 include LowParseExample9.Aux
 open FStar.Tactics.V2
 open Pulse.Lib.Pervasives
+open Pulse.Lib.Slice
 open LowParse.Spec.Base
 
+module SZ = FStar.SizeT
+module R = Pulse.Lib.Reference
+module S = Pulse.Lib.Slice
 module LPS = LowParse.Pulse.Base
 module LPI = LowParse.Pulse.Int
 module LPC = LowParse.Pulse.Combinators
 module PPC = LowParse.PulseParse.Combinators
 module PPS = LowParse.PulseParse.Sum
 module I32 = FStar.Int32
-
-(* Pulse validators for known dsum cases *)
 
 inline_for_extraction noextract
 let pulse_validate_tt_cases (x: dsum_known_key tt_sum)
@@ -30,27 +32,62 @@ let pulse_jump_tt_cases (x: dsum_known_key tt_sum)
   | Kb -> (LPI.jump_u16 <: LPS.jumper (dsnd (parse_tt_cases Kb)))
   | _ -> LPS.jump_constant_size parse_false 0sz
 
-(* validate_t and jump_t — same pattern as Low* using dep_enum_destr_tac *)
+(* Use dep_maybe_enum_destr_t_tac to normalize ALL branches.
+   validate_dsum_cases_dispatch returns validate_dsum_cases_t which
+   has the same pre/post as validator but for parse_dsum_cases'. *)
 
-let validate_t (k: kt) : Tot (LPS.validator (parse_t k)) =
-  lemma_synth_kt_inj ();
-  LPC.validate_synth
-    (PPC.validate_compose_context synth_kt_inv (refine_with_tag key_of_tt)
-      (parse_dsum_cases tt_sum parse_tt_cases parse_u32)
-      (PPS.validate_dsum_cases tt_sum parse_tt_cases pulse_validate_tt_cases LPI.validate_u32
-        (_ by (dep_enum_destr_tac ())))
-      k)
-    (synth_t k)
+inline_for_extraction noextract
+let validate_dcase : (tg: dsum_repr_type tt_sum) -> Tot (PPS.validate_dsum_cases_t tt_sum parse_tt_cases parse_u32 (maybe_enum_key_of_repr (dsum_enum tt_sum) tg))
+= PPS.validate_dsum_cases_dispatch tt_sum parse_tt_cases pulse_validate_tt_cases LPI.validate_u32
+    (_ by (dep_maybe_enum_destr_t_tac ()))
 
-let jump_t (k: kt) : Tot (LPS.jumper (parse_t k)) =
+inline_for_extraction noextract
+let jump_dcase : (tg: dsum_repr_type tt_sum) -> Tot (PPS.jump_dsum_cases_t tt_sum parse_tt_cases parse_u32 (maybe_enum_key_of_repr (dsum_enum tt_sum) tg))
+= PPS.jump_dsum_cases_dispatch tt_sum parse_tt_cases pulse_jump_tt_cases LPI.jump_u32
+    (_ by (dep_maybe_enum_destr_t_tac ()))
+
+(* validate_t as a Pulse fn — maps kt to dsum_key, dispatches, wraps *)
+
+#push-options "--z3rlimit 32"
+
+inline_for_extraction
+fn validate_t
+  (k: kt)
+: LPS.validator (parse_t k)
+=
+  (input: S.slice byte)
+  (poffset: R.ref SZ.t)
+  (#offset: Ghost.erased SZ.t)
+  (#pm: perm)
+  (#v: Ghost.erased bytes)
+{
+  let sinput = Ghost.hide (Seq.slice v (SZ.v offset) (Seq.length v));
   lemma_synth_kt_inj ();
-  LPC.jump_synth
-    (PPC.jump_compose_context synth_kt_inv (refine_with_tag key_of_tt)
-      (parse_dsum_cases tt_sum parse_tt_cases parse_u32)
-      (PPS.jump_dsum_cases tt_sum parse_tt_cases pulse_jump_tt_cases LPI.jump_u32
-        (_ by (dep_enum_destr_tac ())))
-      k)
-    (synth_t k)
+  parse_t_eq k sinput;
+  let mk = synth_kt_inv k;
+  parse_dsum_cases_eq_forall tt_sum parse_tt_cases parse_u32 mk;
+  validate_dcase (repr_of_maybe_enum_key (dsum_enum tt_sum) mk) input poffset
+}
+
+inline_for_extraction
+fn jump_t
+  (k: kt)
+: LPS.jumper (parse_t k)
+=
+  (input: S.slice byte)
+  (offset: SZ.t)
+  (#pm: perm)
+  (#v: Ghost.erased bytes)
+{
+  let sinput = Ghost.hide (Seq.slice v (SZ.v offset) (Seq.length v));
+  lemma_synth_kt_inj ();
+  parse_t_eq k sinput;
+  let mk = synth_kt_inv k;
+  parse_dsum_cases_eq_forall tt_sum parse_tt_cases parse_u32 mk;
+  jump_dcase (repr_of_maybe_enum_key (dsum_enum tt_sum) mk) input offset
+}
+
+#pop-options
 
 fn main ()
   requires emp
